LogicGenerator/demo931/Config - Copy (2).v
@@ -6,44 +6,16 @@ Import ListNotations.
 
 Definition how_connectives :=
   [ primitive_connective join;
-    primitive_connective impp;
+    FROM_model_TO_impp;
     FROM_join_TO_sepcon].
 
 Definition how_judgements :=
-  [ primitive_judgement provable;
-    FROM_provable_TO_derivable1
-  ].
+  [ FROM_model_TO_provable ].
 
 Definition transparent_names :=
-  [provable : parameter].
+  [ provable : parameter].
 
 Definition primitive_rule_classes :=
-  [ provability_OF_sepcon_rule].
-
-(* Definition how_connectives :=
-  [primitive_connective impp
-  ;primitive_connective andp
-  ;primitive_connective sepcon
-  ;FROM_impp_TO_multi_imp
-  ;FROM_empty_set_TO_empty_context
-  ].
-
-Definition how_judgements :=
-  [ primitive_judgement provable
-  ; FROM_provable_TO_derivable
-  ].
-
-Definition transparent_names :=
-  [expr:parameter
-  ;impp:parameter
-  ;andp:parameter
-  ;sepcon:parameter
-  ;provable:parameter].
-
-Definition primitive_rule_classes :=
-  [ provability_OF_impp
-  ; provability_OF_andp
-  ; provability_OF_sepcon_rule_AS_weak
-  ; provability_OF_sepcon_rule_AS_mono
-  ]. *)
-
+  [ join_is_SA ].
+  
+  
