LogicGenerator/demo931/Interface.v
@@ -37,9 +37,6 @@ Parameter Inline tree_pos : Type .
   Axiom sepcon_comm_impp : (forall x y : expr, provable (impp (sepcon x y) (sepcon y x))) .
   Axiom sepcon_assoc1 : (forall x y z : expr, provable (impp (sepcon x (sepcon y z)) (sepcon (sepcon x y) z))) .
   Axiom sepcon_mono : (forall x1 x2 y1 y2 : expr, provable (impp x1 x2) -> provable (impp y1 y2) -> provable (impp (sepcon x1 y1) (sepcon x2 y2))) .
-  Axiom sepcon_comm_impp : (forall x y : expr, provable (impp (sepcon x y) (sepcon y x))) .
-  Axiom sepcon_assoc1 : (forall x y z : expr, provable (impp (sepcon x (sepcon y z)) (sepcon (sepcon x y) z))) .
-  Axiom sepcon_mono : (forall x1 x2 y1 y2 : expr, provable (impp x1 x2) -> provable (impp y1 y2) -> provable (impp (sepcon x1 y1) (sepcon x2 y2))) .
   Axiom sepcon_proper_impp : (Morphisms.Proper (Morphisms.respectful (fun x y : expr => provable (impp x y)) (Morphisms.respectful (fun x y : expr => provable (impp x y)) (fun x y : expr => provable (impp x y)))) sepcon) .
   Axiom expr_deep : Set .
   Axiom impp_deep : (expr_deep -> expr_deep -> expr_deep) .
@@ -104,12 +101,9 @@ Include Rules.
   Instance sepconFJ : (SepconDefinition_Join Join2Sepcon) := Join2Sepcon_Normal .
   Instance provableDef_model : (ProvableDefinition_Model GammaP_modelL) := Model2Provable_Normal .
 (* aux derived instances *)
-  Instance sepconAX_modelL : (SepconAxiomatization Model_L GammaP_modelL) := SeparationAlgebra2SepconAxiomatization .
+  Instance sepconAX : (SepconAxiomatization L GammaP) := SeparationAlgebra2SepconAxiomatization .
 Definition tree_pos : Type := tree_pos.
 (* derived rules *)
-  Definition sepcon_comm_impp : (forall x y : expr, provable (impp (sepcon x y) (sepcon y x))) := sepcon_comm_impp .
-  Definition sepcon_assoc1 : (forall x y z : expr, provable (impp (sepcon x (sepcon y z)) (sepcon (sepcon x y) z))) := sepcon_assoc1 .
-  Definition sepcon_mono : (forall x1 x2 y1 y2 : expr, provable (impp x1 x2) -> provable (impp y1 y2) -> provable (impp (sepcon x1 y1) (sepcon x2 y2))) := sepcon_mono .
   Definition sepcon_comm_impp : (forall x y : expr, provable (impp (sepcon x y) (sepcon y x))) := sepcon_comm_impp .
   Definition sepcon_assoc1 : (forall x y z : expr, provable (impp (sepcon x (sepcon y z)) (sepcon (sepcon x y) z))) := sepcon_assoc1 .
   Definition sepcon_mono : (forall x1 x2 y1 y2 : expr, provable (impp x1 x2) -> provable (impp y1 y2) -> provable (impp (sepcon x1 y1) (sepcon x2 y2))) := sepcon_mono .
